merge e05 material

uw-cse-505/e05/E05_OpSemProofs.v
@@ -1,12 +1,65 @@
 (** * Episode 05: Proofs About Operational Semantics *)
 
+Require Import List.
 Require Import String.
+Require Import ZArith.
+
+(** use fancy string notations *)
 Open Scope string.
+
+(** we'll use a binary representation of signed integers *)
+Print Z.
+Print positive.
+
+Set Implicit Arguments.
+
+(** quick review of fold *)
+Fixpoint fold A B (f: A -> B -> B)
+                  (l: list A) (b: B) :=
+  match l with
+    | nil => b
+    | x :: xs => f x (fold f xs b)
+  end.
+
+(** "+" can mean different things in different scopes *)
+Locate "+".
+
+Fixpoint countdown (n: nat) :=
+  match n with
+    | O => nil
+    | S m => Z_of_nat n :: countdown m
+  end.
+
+Eval cbv in (countdown 5).
+Eval cbv in (fold Z.add (countdown 5) 0%Z).
+Eval cbv in (fold Z.add (countdown 12) 0%Z).
+
+(**
+<<
+ fold + (3 :: 2 :: 1 :: nil) 0
+     ==> 3 + (2 + (1 + 0))
+>>
+*)
+
+(** Defining [fact] with an anonymous [fix] (note the type!): *)
+Definition fact : nat -> nat :=
+  fix loop (n: nat) :=
+      match n with
+        | O => 1
+        | S m => n * loop m
+      end.
+
+(** Could have also defined [fact] using [Fixpoint]:
+<<
+Fixpoint fact (n: nat) : nat := ...
+>>
+*)
+
 
 (** AST *)
 
 Definition var := string.
-Definition val := nat.
+Definition val := Z.
 
 Inductive expr : Type :=
 | Const : val -> expr
@@ -21,36 +74,62 @@ Inductive stmt : Type :=
 | Cond : expr -> stmt -> stmt -> stmt
 | While : expr -> stmt -> stmt.
 
-(** Small Step Operational Semantics *)
+(** switch to association lists for heaps *)
+Definition heap := list (var * val).
 
-Definition heap := var -> val.
+Fixpoint lkup (k: var) (h: heap) :=
+  match h with
+    | nil => 0%Z
+    | (x, v) :: h' =>
+      if string_dec k x then v else lkup k h'
+  end.
+
+(** fancy type containing proofs, but that acts like a [bool] *)
+Check string_dec.
+(**
+<<
+string_dec
+     : forall s1 s2 : string,
+       {s1 = s2} + {s1 <> s2}
+>>
+*)
 
 Definition empty : heap :=
-  fun s => 0.
+  nil.
 
-Definition add_binding n v h : heap :=
-  fun s => if string_dec s n then v else h s.
-
+(** Small Step Operational Semantics *)
 Inductive Eval (h: heap) : expr -> val -> Prop :=
 | EConst : forall n,
   Eval h (Const n) n
 | EVar : forall x,
-  Eval h (Var x) (h x)
+  Eval h (Var x) (lkup x h)
 | EAdd : forall e1 e2 c1 c2 c3,
   Eval h e1 c1 ->
   Eval h e2 c2 ->
-  c3 = c1 + c2 ->
+  c3 = (c1 + c2)%Z ->
   Eval h (Add e1 e2) c3
 | EMul : forall e1 e2 c1 c2 c3,
   Eval h e1 c1 ->
   Eval h e2 c2 ->
-  c3 = c1 * c2 ->
+  c3 = (c1 * c2)%Z ->
   Eval h (Mul e1 e2) c3.
 
-Inductive Step (h : heap) : stmt -> heap -> stmt -> Prop :=
+(** not every [(heap, expr, Z)] is related by [Eval] *)
+Lemma not_in_eval:
+  forall x,
+  Eval nil (Var x) 1%Z -> False.
+Proof.
+  intros. inversion H.
+Qed.
+
+(** the [Eval] relation has nothing to do with [Eval] command *)
+Eval cbv in (countdown 5).
+
+Inductive Step (h : heap)
+ : stmt -> heap -> stmt -> Prop :=
 | SAssign : forall e c x,
   Eval h e c ->
-  Step h (Assign x e) (fun s => if string_dec s x then c else h s) Skip
+  Step h (Assign x e) ((x, c) :: h) Skip
 | SSeq1 : forall s,
   Step h (Seq Skip s) h s
 | SSeq2 : forall s1 s2 s1' h',
@@ -58,21 +137,46 @@ Inductive Step (h : heap) : stmt -> heap -> stmt -> Prop :=
   Step h (Seq s1 s2) h' (Seq s1' s2)
 | SCondT : forall e c s1 s2,
   Eval h e c ->
-  c > 0 ->
+  (c > 0)%Z ->
   Step h (Cond e s1 s2) h s1
 | SCondF : forall e c s1 s2,
   Eval h e c ->
-  c <= 0 ->
+  (c <= 0)%Z ->
   Step h (Cond e s1 s2) h s2
 | SWhileT : forall e c s,
   Eval h e c ->
-  c > 0 ->
+  (c > 0)%Z ->
   Step h (While e s) h (Seq s (While e s))
 | SWhileF : forall e c s,
   Eval h e c ->
-  c <= 0 ->
+  (c <= 0)%Z ->
   Step h (While e s) h Skip.
+
+Inductive StepN : heap -> stmt -> nat ->
+                  heap -> stmt -> Prop :=
+| StepN_refl: forall h s,
+  StepN h s O h s
+| StepN_step: forall h s n h' s' h'' s'',
+  Step h s h' s' ->
+  StepN h' s' n h'' s'' ->
+  StepN h s (S n) h'' s''.
 
 (** Divergance *)
 
-(** No Negatives *)
+Lemma diverges1:
+  forall h n, exists h', exists s',
+  StepN h (While (Const 1%Z) Skip) n h' s'.
+Proof.
+Admitted.
+(*
+  intros.
+  induction n.
+  { exists h.
+    exists (While (Const 1%Z) Skip).
+    apply StepN_refl. (* constructor. *)
+  }
+  { firstorder. rename x into h'.
+    rename x0 into s'. exists h.
+    eexists. eapply StepN_step.
+    ... stuck! ...
+*)
